---
id: nyx4l2y9q6mt3rpoqd63l4f
title: Demostrations
desc: ''
updated: 1702756790194
created: 1702755930253
---

## $\forall{ n } \in \mathbb{ N }^*$ satisfied that $\sum_{ i = 0 }^n { 2^i } = 2^{ n - 1 } - 1$

- Base case.

	$$
	\sum_{ i = 0 }^{ n = 0 } { 2^i } = 2^{ n + 1 } - 1 \quad 2^0 = 2^{ 0 + 1 } - 1 \quad 1 = 1
		$$

- Induction case.

	$$
	\sum_{ i = n + 1 }^{ n + 1 } { 2^i } = 2^{ (n + 1) + 1 } - 1 \quad 2^0 + 2^1 + \dots + 2^n + 2^{ n + 1 } = 2^{ n + 2 } - 1 \\[10 pt]

	\underbrace{2^{ n + 1 } - 1}_{2^0 + 2^1 + \dots + 2^n} + 2^{ n + 1 } = (2^{ n + 1 } + 2^{ n + 1 }) - 1 = 2^{ n + 1 } (1 + 1) - 1 = 2^{ n + 2 } - 1
	$$

## $\forall{ n } \in \mathbb{ N }^*$ satisfied that $\sum_{ k = 1 }^n k = \frac{ n (n + 1) }{ 2 }$ (arithmetic series)

## $\forall{ n } \in \mathbb{ N }^*$ satisfied that $\sum_{ k = 1 }^n k^2 = \frac{ n (n + 1) (2n + 1) }{ 6 }$ (square series)

## $\forall{ n } \in \mathbb{ N }^*$ satisfied that $\sum_{ k = 1 }^n k^3 = \frac{ n^2 (n + 1)^2 }{ 4 }$ (cube series)

## $\forall{ n } \in \mathbb{ N }^*$ satisfied that $\sum_{ k = 0 }^n x^k = \frac{ x^{ n + 1 } - 1 }{ x - 1 }$ (geometric series)

## $\forall{ n } \in \mathbb{ N }^*$ satisfied that $\sum_{ k = 0 }^\infty x^k = \frac{ 1 }{ 1 - x } \quad |x| < 1$ (geometric series)

## $\forall{ n } \in \mathbb{ N }^*$ satisfied that $\sum_{k = 1}^{n} \frac{1}{k} = \ln n +$ (harmonic series)
